theories/Cbor/Encoding.v
@@ -1,0 +1,172 @@
+From Coq Require Import FunInd.
+From Coq Require Import funind.Recdef.
+From Coq Require Import Lists.List.
+                 Import ListNotations.
+From Coq Require Import Strings.Ascii.
+From Coq Require Import Strings.String.
+From Coq Require Import ZArith.
+
+From CoqUplc Require Import Prelude.Bytes.
+From CoqUplc Require Import Prelude.FunctionalNotations.
+From CoqUplc Require Import Prelude.Option.
+
+From CoqUplc Require Import PlutusV3.Uplc.
+
+Local Open Scope bool_scope.
+Local Open Scope N_scope.
+Local Open Scope functional_scope.
+
+Local Definition string_cons (x y : string) : string := concat "" [x; y].
+Local Notation "x ⋅ y" := (string_cons x y) (at level 99).
+
+
+Local Definition b_ (i n : N) : ascii :=
+  let p := N.pow 256 i in
+  ascii_of_N (N.div n p).
+
+Local Definition e_1 (n : N) : list ascii := [b_ 0 n].
+Local Definition e_2 (n : N) : list ascii := [b_ 1 n; b_ 0 n].
+Local Definition e_4 (n : N) : list ascii := [b_ 3 n; b_ 2 n; b_ 1 n; b_ 0 n].
+Local Definition e_8 (n : N) : list ascii := [b_ 7 n; b_ 6 n; b_ 5 n; b_ 4 n; b_ 3 n; b_ 2 n; b_ 1 n; b_ 0 n].
+
+Local Example e_8_ex1 : string_of_list_ascii (e_8 7234295460216005990) = "deadbeef"%string. Proof eq_refl.
+
+
+Local Definition head_first_byte (m n : N) : ascii :=
+  ascii_of_N (32 * m + n).
+
+Local Definition encode_head (m n : N) : option string :=
+  let fb := head_first_byte m in
+  if m <=? 7 then
+         if n <=?                   23 then Some (string_of_list_ascii [fb n])
+    else if n <=?                  255 then Some (string_of_list_ascii (fb 24 :: e_1 n))
+    else if n <=?                65535 then Some (string_of_list_ascii (fb 25 :: e_2 n))
+    else if n <=?           4294967295 then Some (string_of_list_ascii (fb 26 :: e_4 n))
+    else if n <=? 18446744073709551615 then Some (string_of_list_ascii (fb 27 :: e_8 n))
+    else None
+  else None.
+
+
+Local Open Scope nat_scope.
+
+Local Lemma length_substing_le : forall (s : string) (n m : nat), length (substring n m s) <= length s.
+  induction s; induction m; induction n; simpl; auto with arith.
+Qed.
+
+Function split_to_chunks (s : string) {measure length s} : list string :=
+  match s with
+  | String a s' => substring 0 64 s :: split_to_chunks (substring 64 (length s) s)
+  | EmptyString => []
+  end.
+Proof.
+  intros s a s' Hs; simpl; unfold lt; apply le_n_S; apply length_substing_le.
+Defined.
+
+Local Close Scope nat_scope.
+
+Local Example split_to_chunks_ex1 : split_to_chunks "1234567890123456789012345678901234567890123456789012345678901234"%string =
+  [ "1234567890123456789012345678901234567890123456789012345678901234"%string ]. Proof eq_refl.
+Local Example split_to_chunks_ex2 : split_to_chunks "12345678901234567890123456789012345678901234567890123456789012345"%string =
+  [ "1234567890123456789012345678901234567890123456789012345678901234"%string
+  ; "5"%string
+  ]. Proof eq_refl.
+Local Example split_to_chunks_ex3 : split_to_chunks "1234567890123456789012345678901234567890123456789012345678901234123456789012345678901234567890123456789012345678901234567890123456"%string =
+  [ "1234567890123456789012345678901234567890123456789012345678901234"%string
+  ; "1234567890123456789012345678901234567890123456789012345678901234"%string
+  ; "56"%string
+  ]. Proof eq_refl.
+
+
+Local Definition encode_indef (m : N) : ascii := head_first_byte m 31.
+
+Local Definition encode_bytestring_chunk (s : string) : option string :=
+  option_map (fun h => string_cons h s) (encode_head 2 (length s |> N.of_nat)).
+
+Local Definition list_of_option {A : Type}  (x : option A) : list A :=
+  match x with
+  | Some v => [v]
+  | None   => []
+  end.
+
+Local Definition encode_bytestring (s : string) : option string :=
+  match split_to_chunks s with
+  | []      => Some ""%string
+  | h :: [] => encode_bytestring_chunk h
+  | chunks  => Some (concat "" (string_of_list_ascii [encode_indef 2] :: flat_map (encode_bytestring_chunk >> list_of_option) chunks ++ [string_of_list_ascii ["255"%char]]))
+  end.
+
+Local Example encode_bytestring_ex1 : encode_bytestring "1234567890123456789012345678901234567890123456789012345678901234"%string =
+  Some (concat "" [ string_of_list_ascii ["088"%char; "064"%char]; "1234567890123456789012345678901234567890123456789012345678901234"%string]). Proof eq_refl.
+Local Example encode_bytestring_ex2 : encode_bytestring "12345678901234567890123456789012345678901234567890123456789012345"%string =
+  Some (concat "" [ string_of_list_ascii ["095"%char]
+                  ; string_of_list_ascii ["088"%char; "064"%char]; "1234567890123456789012345678901234567890123456789012345678901234"%string
+                  ; string_of_list_ascii ["065"%char]; "5"%string
+                  ; string_of_list_ascii ["255"%char]
+                  ]). Proof eq_refl.
+Local Example encode_bytestring_ex3 : encode_bytestring "1234567890123456789012345678901234567890123456789012345678901234123456789012345678901234567890123456789012345678901234567890123456"%string =
+  Some (concat "" [ string_of_list_ascii ["095"%char]
+                  ; string_of_list_ascii ["088"%char; "064"%char]; "1234567890123456789012345678901234567890123456789012345678901234"%string
+                  ; string_of_list_ascii ["088"%char; "064"%char]; "1234567890123456789012345678901234567890123456789012345678901234"%string
+                  ; string_of_list_ascii ["066"%char]; "56"%string
+                  ; string_of_list_ascii ["255"%char]
+                  ]). Proof eq_refl.
+
+Local Open Scope Z_scope.
+
+Local Definition encode_Z (n : Z) : option string :=
+       if (                    0 <=? n) && (n <=?  18446744073709551615) then encode_head 0 (Z.to_N n)
+  else if ( 18446744073709551616 <=? n                                 ) then option_flatmap2 (string_cons >>> Some) (encode_head 6 2) (n |> Z.to_N |> bytestring_of_N_be |> encode_bytestring)
+  else if (-18446744073709551616 <=? n) && (n <=?                    -1) then encode_head 1 ((-n - 1) |> Z.to_N)
+  else if (                                 n <=? -18446744073709551617) then option_flatmap2 (string_cons >>> Some) (encode_head 6 3) ((-n - 1) |> Z.to_N |> bytestring_of_N_be |> encode_bytestring)
+  else None.
+
+
+Local Definition encode_ctag (i : Z) : option string :=
+       if (0 <=? i) && (i <=?   6) then encode_head 6 (121 + i |> Z.to_N)
+  else if (7 <=? i) && (i <=? 127) then encode_head 6 (1280 + (i - 7) |> Z.to_N)
+  else option_flatmap3 ((string_cons >>> string_cons) >>>> Some) (encode_head 6 102) (encode_head 4 2) (encode_Z i).
+
+Fixpoint encode_data (d : data) {struct d} : option string :=
+  match d with
+  | DataConstr i l =>
+      let l_e := flat_map (encode_data >> list_of_option) l in
+      option_map (fun e_ctag => concat "" (e_ctag :: [string_of_list_ascii [encode_indef 4]] ++ l_e ++ [string_of_list_ascii ["255"%char]])) (encode_ctag i)
+  | Map        l   =>
+      let l_e := flat_map (fun p => option_flatmap2 (string_cons >>> Some) (encode_data (fst p)) (encode_data (snd p)) |> list_of_option) l in
+      option_map (fun h => concat "" (h :: l_e)) (encode_head 5 (List.length l |> N.of_nat))
+  | DataList   l   =>
+      let l_e := flat_map (encode_data >> list_of_option) l in
+      Some (concat "" (string_of_list_ascii [encode_indef 4] :: l_e ++ [string_of_list_ascii ["255"%char]]))
+  | I          n   => encode_Z n
+  | B          s   => encode_bytestring s
+  end.
+
+From Coq Require Import Init.Byte.
+
+
+Local Definition of_hexstring (bs : list byte) : string :=
+  map ascii_of_byte bs |> string_of_list_ascii.
+
+Local Example encode_data_exZ1 : encode_data (I 12) = Some (string_of_list_ascii ["012"%char]). Proof eq_refl.
+Local Example encode_data_exZ2 : encode_data (I 42) = Some (string_of_list_ascii ["024"%char; "042"%char]). Proof eq_refl.
+
+Local Example encode_data_ex1 :
+    encode_data (
+      DataConstr 0 [
+        DataConstr 0 [I 1284531];
+        I 1739713998000
+      ]
+    ) = Some (of_hexstring [ xd8; x79; x9f; xd8; x79; x9f; x1a; x00; x13; x99; xb3; xff
+                           ; x1b; x00; x00; x01; x95; x0f; x08; xec; xb0; xff]).
+Proof eq_refl.
+
+Local Example encode_data_ex2 :
+  encode_data (
+    DataConstr 0 [
+      I 144375414;
+      I 22710;
+      I 4387720097
+    ]
+  ) = Some (of_hexstring [xd8; x79; x9f; x1a; x08; x9a; xfe; x76; x19; x58; xb6; x1b; x00; x00; x00; x01; x05; x87; x4b; xa1; xff]).
+Proof eq_refl.
+
