theories/Examples/Examples02.v
@@ -1,0 +1,104 @@
+From Coq Require Import Lists.List.
+                 Import ListNotations.
+From Coq Require Import Strings.Ascii.
+From Coq Require Import Strings.Byte.
+From Coq Require Import Strings.String.
+From Coq Require Import ZArith.
+
+From CoqUplc Require Import Unicode.String.
+From CoqUplc Require Import Unicode.StringShow.
+
+From CoqUplc Require Import PlutusV3.CekMachine.
+From CoqUplc Require Import PlutusV3.CekValue.
+From CoqUplc Require Import PlutusV3.Uplc.
+
+Local Open Scope string_scope.
+Local Open Scope Z_scope.
+
+Module ExampleNotations.
+  Definition const_of_bytes (b : list byte) : const := ByteString (string_of_list_ascii (map ascii_of_byte b)).
+  
+  Declare Scope exampleNotation_scope.
+  Delimit Scope exampleNotation_scope with exampleNotation.
+
+  Notation "'plutusV3' x"          := (Program (Version 1 1 0) x)    (at level 89, left associativity) : exampleNotation_scope.
+
+  Notation "'\' x '=>' y"          := (Lam x y)                      (at level 89) : exampleNotation_scope.
+  Notation "'\' x '\' y '=>' z"    := (Lam x (Lam y z))              (at level 89) : exampleNotation_scope.
+  Notation "x '#' y"               := (Apply x y)                    (at level 88, left associativity) : exampleNotation_scope.
+  Notation "'val' x '<-' y 'in' z" := (Apply (Lam x z) y)            (at level 89) : exampleNotation_scope.
+  Notation "'value' x"             := (Var x)                        (at level 87) : exampleNotation_scope.
+  
+  Notation "'byteStringToInteger'" := (Builtin ByteStringToInteger)  (at level 87) : exampleNotation_scope.
+  Notation "'decodeUtf8'"          := (Builtin DecodeUtf8)           (at level 87) : exampleNotation_scope.
+  Notation "'expMod'"              := (Builtin ExpModInteger)        (at level 87) : exampleNotation_scope.
+  Notation "'findFirstSetBit'"     := (Builtin FindFirstSetBit)      (at level 87) : exampleNotation_scope.
+  Notation "'integerToByteString'" := (Builtin IntegerToByteString)  (at level 87) : exampleNotation_scope.
+  Notation "'replicateByte'"       := (Builtin ReplicateByte)        (at level 87) : exampleNotation_scope.
+  Notation "'serialiseData'"       := (Builtin SerialiseData)        (at level 87) : exampleNotation_scope.
+  Notation "'trace'"               := (Force (Builtin Trace))        (at level 87) : exampleNotation_scope.
+  Notation "'writeBits'"           := (Builtin WriteBits)            (at level 87) : exampleNotation_scope.
+  
+  Notation "'t'"                   := (Const (Bool true))            (at level 87) : exampleNotation_scope.
+  Notation "'con' x"               := (Const x)                      (at level 87) : exampleNotation_scope.
+  Notation "'int' x"               := (Integer x)                    (at level 86) : exampleNotation_scope.
+  Notation "'bytes' x"             := (const_of_bytes x)             (at level 86) : exampleNotation_scope.
+  Notation "'data' x"              := (Data x)                       (at level 86) : exampleNotation_scope.
+  Notation "'clist' x"             := (ConstList x)                  (at level 86) : exampleNotation_scope.
+
+  Notation "'success' x"           := (Halt (VCon x), [])            (at level 89) : exampleNotation_scope.
+  Notation "'succ:' x 'trace:' y"  := (Halt (VCon x), [y])           (at level 89) : exampleNotation_scope.
+End ExampleNotations.
+
+Import ExampleNotations.
+
+Local Open Scope exampleNotation_scope.
+
+(* serialiseData: batch 2 function *)
+Definition serialiseData_program : program := plutusV3
+  \"d" => serialiseData # value "d".
+
+Example example_data :=
+  DataList [ DataList [I 0; I 0; I 0; I 0; I 0]
+           ; I 17
+           ].
+
+Property serialiseData_example :
+    cek_execute_program serialiseData_program [con data example_data] 11 = success bytes [x9f; x9f; x00; x00; x00; x00; x00; xff; x11; xff].
+Proof.
+  compute. reflexivity.
+Qed.
+
+
+(* byteStringToInteger, integerToByteString: batch 4 function *)
+Definition I_to_B_to_I_program : program := plutusV3
+  \"i" =>
+      val "b" <- integerToByteString # t # con int 7 # value "i" in
+      trace # (decodeUtf8 # value "b") # (byteStringToInteger # t # value "b").
+
+Property i_b_i_example :
+  cek_execute_program I_to_B_to_I_program [con int 22637249857680191] 46 = succ: int 22637249857680191 trace: "Plutus?"%unicode.
+Proof.
+  compute. reflexivity.
+Qed.
+
+
+(* findFirstSetBit, replicateByte, writeBits: batch 5 functions *)
+Definition find_first_index_program : program := plutusV3
+  \"l" \"xs" =>
+      val "bs" <- writeBits # (replicateByte # value "l" # con int 0) # value "xs" # t in
+      findFirstSetBit # value "bs".
+
+Property find_first_example :
+    cek_execute_program find_first_index_program [con int 4; con clist [int 15; int 4]] 41 = success int 4.
+Proof.
+  compute. reflexivity.
+Qed.
+
+
+Definition expMod_program : program :=
+  plutusV3 \"a" \"e" => expMod # value "a" # value "e" # con int 256.
+
+Property expMod_example :
+    cek_execute_program expMod_program [con int 2; con int 8] 24 = success int 0.
+Proof eq_refl.
