theories/PlutusV3/BuiltinFunctions/ByteString.v
@@ -1,0 +1,171 @@
+From Coq Require Import Lists.List.
+                 Import ListNotations.
+From Coq Require Import Strings.Ascii.
+From Coq Require Import Strings.String.
+From Coq Require Import ZArith.
+
+From CoqUplc Require Import Prelude.Bytes.
+From CoqUplc Require Import Prelude.FunctionalNotations.
+From CoqUplc Require Import Prelude.Option.
+
+From CoqUplc Require Import PlutusV3.CekValue.
+From CoqUplc Require Import PlutusV3.Uplc.
+
+Local Open Scope string_scope.
+Local Open Scope functional_scope.
+
+Definition appendByteString (Vs : list cekValue) : option cekValue :=
+   match Vs with
+   | [VCon (ByteString x); VCon (ByteString y)] => append x y |> cekValue_of_byteString |> Some
+   | _                                          => None
+   end.
+
+Definition consByteString_variant1 (Vs : list cekValue) : option cekValue :=
+   match Vs with
+   | [VCon (Integer x); VCon (ByteString y)] => match Z.modulo x 256 with
+                                                | Z0     => String.String Ascii.zero             y |> cekValue_of_byteString |> Some
+                                                | Zpos p => String.String (Ascii.ascii_of_pos p) y |> cekValue_of_byteString |> Some
+                                                | Zneg p => None (* impossible case *)
+                                                end
+   | _                                       => None
+   end.
+
+Definition consByteString_variant2 (Vs : list cekValue) : option cekValue :=
+   match Vs with
+   | [VCon (Integer Z0      ); VCon (ByteString y)] => String.String Ascii.zero y |> cekValue_of_byteString |> Some
+   | [VCon (Integer (Zpos p)); VCon (ByteString y)] => if (p <=? 255)%positive
+                                                         then String.String (Ascii.ascii_of_pos p) y |> cekValue_of_byteString |> Some
+                                                         else None
+   | _                                              => None
+   end.
+
+Definition sliceByteString (Vs : list cekValue) : option cekValue :=
+  match Vs with
+   | [VCon (Integer i); VCon (Integer l); VCon (ByteString b)] => substring (Z.to_nat i) (Z.to_nat l) b |> cekValue_of_byteString |> Some
+   | _                                                         => None
+   end.
+
+Definition lengthOfByteString (Vs : list cekValue) : option cekValue :=
+  match Vs with
+   | [VCon (ByteString b)] => Z.of_nat (length b) |> cekValue_of_integer |> Some
+   | _                     => None
+   end.
+
+Definition Z_of_ascii (x : ascii) : Z := x |> N_of_ascii |> Z.of_N.
+
+Definition indexByteString (Vs : list cekValue) : option cekValue :=
+  match Vs with
+   | [VCon (Integer Z0      ); VCon (ByteString b)] => String.get 0              b |> option_map (Z_of_ascii >> cekValue_of_integer)
+   | [VCon (Integer (Zpos p)); VCon (ByteString b)] => String.get (Pos.to_nat p) b |> option_map (Z_of_ascii >> cekValue_of_integer)
+   | _                                              => None
+   end.
+
+Definition equalsByteString (Vs : list cekValue) : option cekValue :=
+  match Vs with
+   | [VCon (ByteString x); VCon (ByteString y)] => x =? y |> cekValue_of_boolean |> Some
+   | _                                          => None
+   end.
+
+Definition lessThanByteString (Vs : list cekValue) : option cekValue :=
+  match Vs with
+   | [VCon (ByteString x); VCon (ByteString y)] => x <? y |> cekValue_of_boolean |> Some
+   | _                                          => None
+   end.
+
+Definition lessThanEqualsByteString (Vs : list cekValue) : option cekValue :=
+  match Vs with
+   | [VCon (ByteString x); VCon (ByteString y)] => x <=? y |> cekValue_of_boolean |> Some
+   | _                                          => None
+   end.
+
+Definition integerToByteString (Vs : list cekValue) : option cekValue :=
+  match Vs with
+   | [VCon (Bool e); VCon (Integer w); VCon (Integer n)] => option_map cekValue_of_byteString (integer_to_bytestring e w n)
+   | _                                                   => None
+   end.
+
+Definition byteStringToInteger (Vs : list cekValue) : option cekValue :=
+  match Vs with
+   | [VCon (Bool e); VCon (ByteString s)] => bytestring_to_integer e s |> Z.of_N |> cekValue_of_integer |> Some
+   | _                                    => None
+   end.
+
+Definition andByteString (Vs : list cekValue) : option cekValue :=
+  match Vs with
+   | [VCon (Bool e); VCon (ByteString b1); VCon (ByteString b2)] => and_bytestring e b1 b2 |> cekValue_of_byteString |> Some
+   | _                                                           => None
+   end.
+
+Definition orByteString (Vs : list cekValue) : option cekValue :=
+  match Vs with
+   | [VCon (Bool e); VCon (ByteString b1); VCon (ByteString b2)] => or_bytestring e b1 b2 |> cekValue_of_byteString |> Some
+   | _                                                           => None
+   end.
+
+Definition xorByteString (Vs : list cekValue) : option cekValue :=
+  match Vs with
+   | [VCon (Bool e); VCon (ByteString b1); VCon (ByteString b2)] => xor_bytestring e b1 b2 |> cekValue_of_byteString |> Some
+   | _                                                           => None
+   end.
+
+Definition complementByteString (Vs : list cekValue) : option cekValue :=
+  match Vs with
+   | [VCon (ByteString b)] => xor_bytestring false b (extend_to ""%string (length b) "255"%char) |> cekValue_of_byteString |> Some
+   | _                     => None
+   end.
+
+Definition shiftByteString (Vs : list cekValue) : option cekValue :=
+  match Vs with
+   | [VCon (ByteString b); VCon (Integer Z0      )] => b                                 |> cekValue_of_byteString |> Some
+   | [VCon (ByteString b); VCon (Integer (Zpos p))] => shift_bits_right b (Pos.to_nat p) |> cekValue_of_byteString |> Some
+   | [VCon (ByteString b); VCon (Integer (Zneg p))] => shift_bits_left  b (Pos.to_nat p) |> cekValue_of_byteString |> Some
+   | _                                              => None
+   end.
+
+Definition rotateByteString (Vs : list cekValue) : option cekValue :=
+  match Vs with
+   | [VCon (ByteString b); VCon (Integer Z0      )] => b                                  |> cekValue_of_byteString |> Some
+   | [VCon (ByteString b); VCon (Integer (Zpos p))] => rotate_bits_right b (Pos.to_nat p) |> cekValue_of_byteString |> Some
+   | [VCon (ByteString b); VCon (Integer (Zneg p))] => rotate_bits_left  b (Pos.to_nat p) |> cekValue_of_byteString |> Some
+   | _                                        => None
+   end.
+
+Definition countSetBits (Vs : list cekValue) : option cekValue :=
+  match Vs with
+   | [VCon (ByteString b)] => count_set_bits b |> Z.of_nat |> cekValue_of_integer |> Some
+   | _                     => None
+   end.
+
+Definition findFirstSetBit (Vs : list cekValue) : option cekValue :=
+  match Vs with
+   | [VCon (ByteString b)] => first_set_bit b |> cekValue_of_integer |> Some
+   | _                     => None
+   end.
+
+Definition readBit (Vs : list cekValue) : option cekValue :=
+  match Vs with
+   | [VCon (ByteString b); VCon (Integer Z0      )] => option_map cekValue_of_boolean (read_bit b 0)
+   | [VCon (ByteString b); VCon (Integer (Zpos p))] => option_map cekValue_of_boolean (read_bit b (Pos.to_nat p))
+   | _                                              => None
+   end.
+
+Local Fixpoint list_integer_of_const_list (l : list const) : option (list Z) :=
+  match l with
+  | Integer z :: t => option_map (cons z) (list_integer_of_const_list t)
+  | _         :: t => None
+  | []             => Some []
+  end.
+
+Definition writeBits (Vs : list cekValue) : option cekValue :=
+  match Vs with
+   | [VCon (ByteString b); VCon (ConstList l); VCon (Bool u)] =>
+       let r := option_flatmap (write_bits b u) (list_integer_of_const_list l) in
+       option_map (cekValue_of_byteString) r
+   | _                                                        => None
+   end.
+
+Definition replicateByte (Vs : list cekValue) : option cekValue :=
+  match Vs with
+   | [VCon (Integer l); VCon (Integer b)] => option_map (cekValue_of_byteString) (replicate_bytes l b)
+   | _                                    => None
+   end.
