theories/PlutusV3/BuiltinFunctions/Data.v
@@ -1,0 +1,129 @@
+From Coq Require Import Lists.List.
+                 Import ListNotations.
+
+From CoqUplc Require Import Prelude.FunctionalNotations.
+
+From CoqUplc Require Import Cbor.Encoding.
+From CoqUplc Require Import PlutusV3.CekValue.
+From CoqUplc Require Import PlutusV3.Uplc.
+
+Local Open Scope functional_scope.
+
+Definition chooseData (Vs : list cekValue) : option cekValue :=
+  match Vs with
+  | [VCon (Data (DataConstr _ _)); c; _; _; _; _] => Some c
+  | [VCon (Data (Map        _  )); _; m; _; _; _] => Some m
+  | [VCon (Data (DataList   _  )); _; _; l; _; _] => Some l
+  | [VCon (Data (I          _  )); _; _; _; i; _] => Some i
+  | [VCon (Data (B          _  )); _; _; _; _; b] => Some b
+  | _                                             => None
+  end.
+
+Local Fixpoint list_const_to_list_data (x : list const) {struct x} : option (list data) :=
+  match x with
+  | (Data d) :: t => option_map (cons d) (list_const_to_list_data t)
+  | _        :: _ => None
+  | []            => Some []
+  end.
+
+Definition constrData (Vs : list cekValue) : option cekValue :=
+  match Vs with
+  | [VCon (Integer i); VCon (ConstList xs)] => option_map ((DataConstr i) >> cekValue_of_data) (list_const_to_list_data xs)
+  | _                                       => None
+  end.
+
+Local Fixpoint list_const_to_data_pair (x : list const) {struct x} : option (list (data * data)) :=
+  match x with
+  | (Pair (Data p1) (Data p2)) :: t => option_map (cons (p1, p2)) (list_const_to_data_pair t)
+  | _                          :: _ => None
+  | []                              => Some []
+  end.
+
+Definition mapData (Vs : list cekValue) : option cekValue :=
+  match Vs with
+  | [VCon (ConstList xs)] => option_map (Map >> cekValue_of_data) (list_const_to_data_pair xs)
+  | _                     => None
+  end.
+
+Definition listData (Vs : list cekValue) : option cekValue :=
+  match Vs with
+  | [VCon (ConstList xs)] => option_map (DataList >> cekValue_of_data) (list_const_to_list_data xs)
+  | _                     => None
+  end.
+
+Definition iData (Vs : list cekValue) : option cekValue :=
+  match Vs with
+  | [VCon (Integer i)] => I i |> cekValue_of_data |> Some
+  | _                  => None
+  end.
+
+Definition bData (Vs : list cekValue) : option cekValue :=
+  match Vs with
+  | [VCon (ByteString b)] => B b |> cekValue_of_data |> Some
+  | _                     => None
+  end.
+
+Local Definition list_data_to_list_const (x : list data) : list const := map Data x.
+
+Definition unConstrData (Vs : list cekValue) : option cekValue :=
+  match Vs with
+  | [VCon (Data (DataConstr i xs))] => list_data_to_list_const xs |> ConstList |> cekValue_of_pair (Integer i) |> Some
+  | _                               => None
+  end.
+
+Local Definition data_pair_to_list_const (x : list (data * data)) : list const :=
+  map (fun (x : data * data) => let (p1, p2) := x in Pair (Data p1) (Data p2)) x.
+
+Definition unMapData (Vs : list cekValue) : option cekValue :=
+  match Vs with
+  | [VCon (Data (Map xs))] => data_pair_to_list_const xs |> cekValue_of_list |> Some
+  | _                      => None
+  end.
+
+Definition unListData (Vs : list cekValue) : option cekValue :=
+  match Vs with
+  | [VCon (Data (DataList xs))] => list_data_to_list_const xs |> cekValue_of_list |> Some
+  | _                           => None
+  end.
+
+Definition unIData (Vs : list cekValue) : option cekValue :=
+  match Vs with
+  | [VCon (Data (I i))] => i |> cekValue_of_integer |> Some
+  | _                   => None
+  end.
+
+Definition unBData (Vs : list cekValue) : option cekValue :=
+  match Vs with
+  | [VCon (Data (B b))] => b |> cekValue_of_byteString |> Some
+  | _                   => None
+  end.
+
+Definition equalsData (Vs : list cekValue) : option cekValue :=
+  match Vs with
+  | [VCon (Data d1); VCon (Data d2)] => data_beq d1 d2 |> cekValue_of_boolean |> Some
+  | _                                => None
+  end.
+
+Definition mkPairData (Vs : list cekValue) : option cekValue :=
+  match Vs with
+  | [VCon (Data d1); VCon (Data d2)] => cekValue_of_pair (Data d1) (Data d2) |> Some
+  | _                                => None
+  end.
+
+Definition mkNilData (Vs : list cekValue) : option cekValue :=
+  match Vs with
+  | [VCon Unit] => cekValue_of_list [] |> Some
+  | _           => None
+  end.
+
+Definition mkNilPairData (Vs : list cekValue) : option cekValue :=
+  match Vs with
+  | [VCon Unit] => cekValue_of_list [] |> Some
+  | _           => None
+  end.
+
+Definition serialiseData (Vs : list cekValue) : option cekValue :=
+  match Vs with
+  | [VCon (Data d)] => option_map cekValue_of_byteString (encode_data d)
+  | _               => None
+  end.
