theories/PlutusV3/BuiltinFunctions/Evaluate.v
@@ -1,13 +1,124 @@
+From CoqUplc Require Import Prelude.FunctionalNotations.
+From CoqUplc Require Import Prelude.List.
+From CoqUplc Require Import Prelude.Monad.
+                     Import MonadNotations.
+
 From CoqUplc Require Import PlutusV3.CekValue.
 From CoqUplc Require Import PlutusV3.Uplc.
+From CoqUplc Require Import Unicode.String.
 
 From CoqUplc Require Import PlutusV3.BuiltinFunctions.Bool.
+From CoqUplc Require Import PlutusV3.BuiltinFunctions.ByteString.
+From CoqUplc Require Import PlutusV3.BuiltinFunctions.Data.
 From CoqUplc Require Import PlutusV3.BuiltinFunctions.Integer.
+From CoqUplc Require Import PlutusV3.BuiltinFunctions.List.
+From CoqUplc Require Import PlutusV3.BuiltinFunctions.Misc.
+From CoqUplc Require Import PlutusV3.BuiltinFunctions.Pair.
+From CoqUplc Require Import PlutusV3.BuiltinFunctions.String.
 
-Definition evaluate_builtin_function (b : builtinFun) : list cekValue -> option cekValue :=
+Local Open Scope functional_scope.
+
+Definition evaluate_builtin_function (b : builtinFun) : list cekValue -> writer (list unicodestring) (option cekValue) :=
   match b with
-  | SubtractInteger => subtractInteger
-  | LessThanInteger => lessThanInteger
-  | IfThenElse      => ifThenElse
-  | _               => fun _ => None
+  (* -- Integer *)
+  | AddInteger               => addInteger               >> mreturn
+  | SubtractInteger          => subtractInteger          >> mreturn
+  | MultiplyInteger          => multiplyInteger          >> mreturn
+  | DivideInteger            => divideInteger            >> mreturn
+  | ModInteger               => modInteger               >> mreturn
+  | QuotientInteger          => quotientInteger          >> mreturn
+  | RemainderInteger         => remainderInteger         >> mreturn
+  | EqualsInteger            => equalsInteger            >> mreturn
+  | LessThanInteger          => lessThanInteger          >> mreturn
+  | LessThanEqualsInteger    => lessThanEqualsInteger    >> mreturn
+  (* -- Bytestring *)
+  | AppendByteString         => appendByteString         >> mreturn
+  | ConsByteString           => consByteString_variant2  >> mreturn (* TODO: verify if it is variant 2 on chain *)
+  | SliceByteString          => sliceByteString          >> mreturn
+  | LengthOfByteString       => lengthOfByteString       >> mreturn
+  | IndexByteString          => indexByteString          >> mreturn
+  | EqualsByteString         => equalsByteString         >> mreturn
+  | LessThanByteString       => lessThanByteString       >> mreturn
+  | LessThanEqualsByteString => lessThanEqualsByteString >> mreturn
+  (* -- Cryptography *)
+  | Sha2_256                 => fun _ => mreturn None
+  | Sha3_256                 => fun _ => mreturn None
+  | Blake2b_256              => fun _ => mreturn None
+  | VerifyEd25519Signature   => fun _ => mreturn None
+  (* -- String *)
+  | AppendString             => appendString             >> mreturn
+  | EqualsString             => equalsString             >> mreturn
+  | EncodeUtf8               => encodeUtf8               >> mreturn
+  | DecodeUtf8               => decodeUtf8               >> mreturn
+  (* -- Bool *)
+  | IfThenElse               => ifThenElse               >> mreturn
+  (* -- Misc *)
+  | ChooseUnit               => chooseUnit               >> mreturn
+  | Trace                    => trace
+  (* -- Pair *)
+  | FstPair                  => fstPair                  >> mreturn
+  | SndPair                  => sndPair                  >> mreturn
+  (* -- List *)
+  | ChooseList               => chooseList               >> mreturn
+  | MkCons                   => mkCons                   >> mreturn
+  | HeadList                 => headList                 >> mreturn
+  | TailList                 => tailList                 >> mreturn
+  | NullList                 => nullList                 >> mreturn
+  (* -- Data *)
+  | ChooseData               => chooseData               >> mreturn
+  | ConstrData               => constrData               >> mreturn
+  | MapData                  => mapData                  >> mreturn
+  | ListData                 => listData                 >> mreturn
+  | IData                    => iData                    >> mreturn
+  | BData                    => bData                    >> mreturn
+  | UnConstrData             => unConstrData             >> mreturn
+  | UnMapData                => unMapData                >> mreturn
+  | UnListData               => unListData               >> mreturn
+  | UnIData                  => unIData                  >> mreturn
+  | UnBData                  => unBData                  >> mreturn
+  | EqualsData               => equalsData               >> mreturn
+  | MkPairData               => mkPairData               >> mreturn
+  | MkNilData                => mkNilData                >> mreturn
+  | MkNilPairData            => mkNilPairData            >> mreturn
+  | SerialiseData            => serialiseData            >> mreturn
+  (* -- Cryptography *)
+  | VerifyEcdsaSecp256k1Signature   => fun _ => mreturn None
+  | VerifySchnorrSecp256k1Signature => fun _ => mreturn None
+  | Bls12_381_G1_add                => fun _ => mreturn None
+  | Bls12_381_G1_neg                => fun _ => mreturn None
+  | Bls12_381_G1_scalarMul          => fun _ => mreturn None
+  | Bls12_381_G1_equal              => fun _ => mreturn None
+  | Bls12_381_G1_hashToGroup        => fun _ => mreturn None
+  | Bls12_381_G1_compress           => fun _ => mreturn None
+  | Bls12_381_G1_uncompress         => fun _ => mreturn None
+  | Bls12_381_G2_add                => fun _ => mreturn None
+  | Bls12_381_G2_neg                => fun _ => mreturn None
+  | Bls12_381_G2_scalarMul          => fun _ => mreturn None
+  | Bls12_381_G2_equal              => fun _ => mreturn None
+  | Bls12_381_G2_hashToGroup        => fun _ => mreturn None
+  | Bls12_381_G2_compress           => fun _ => mreturn None
+  | Bls12_381_G2_uncompress         => fun _ => mreturn None
+  | Bls12_381_millerLoop            => fun _ => mreturn None
+  | Bls12_381_mulMlResult           => fun _ => mreturn None
+  | Bls12_381_finalVerify           => fun _ => mreturn None
+  | Keccak_256                      => fun _ => mreturn None
+  | Blake2b_224                     => fun _ => mreturn None
+  (* -- ByteString *)
+  | IntegerToByteString      => integerToByteString      >> mreturn
+  | ByteStringToInteger      => byteStringToInteger      >> mreturn
+  | AndByteString            => andByteString            >> mreturn
+  | OrByteString             => orByteString             >> mreturn
+  | XorByteString            => xorByteString            >> mreturn
+  | ComplementByteString     => complementByteString     >> mreturn
+  | ShiftByteString          => shiftByteString          >> mreturn
+  | RotateByteString         => rotateByteString         >> mreturn
+  | CountSetBits             => countSetBits             >> mreturn
+  | FindFirstSetBit          => findFirstSetBit          >> mreturn
+  | ReadBit                  => readBit                  >> mreturn
+  | WriteBits                => writeBits                >> mreturn
+  | ReplicateByte            => replicateByte            >> mreturn
+  (* -- Cryptography *)
+  | Ripemd_160               => fun _ => mreturn None
+  (* -- Integer *)
+  | ExpModInteger            => expModInteger            >> mreturn
   end.
