theories/PlutusV3/BuiltinFunctions/Integer.v
@@ -2,19 +2,115 @@ From Coq Require Import Lists.List.
                  Import ListNotations.
 From Coq Require Import ZArith.
 
+From CoqUplc Require Import Prelude.FunctionalNotations.
+
 From CoqUplc Require Import PlutusV3.CekValue.
 From CoqUplc Require Import PlutusV3.Uplc.
 
 Local Open Scope Z_scope.
+Local Open Scope functional_scope.
+
+Definition addInteger (Vs : list cekValue) : option cekValue :=
+   match Vs with
+   | [VCon (Integer x); VCon (Integer y)] => Some (cekValue_of_integer (x + y))
+   | _                                    => None
+   end.
 
 Definition subtractInteger (Vs : list cekValue) : option cekValue :=
    match Vs with
-   | [VCon (Integer x); VCon (Integer y)] => Some (VCon (Integer (x - y)))
+   | [VCon (Integer x); VCon (Integer y)] => Some (cekValue_of_integer (x - y))
+   | _                                    => None
+   end.
+
+Definition multiplyInteger (Vs : list cekValue) : option cekValue :=
+   match Vs with
+   | [VCon (Integer x); VCon (Integer y)] => Some (cekValue_of_integer (x * y))
+   | _                                    => None
+   end.
+
+Definition divideInteger (Vs : list cekValue) : option cekValue :=
+   match Vs with
+   | [VCon (Integer a); VCon (Integer 0)] => None
+   | [VCon (Integer a); VCon (Integer b)] => let d := Z.abs (Z.div a b) in
+                                             match a >=? 0, b >=? 0 with
+                                             | true , true  => d
+                                             | false, true  => -d
+                                             | true , false => -d
+                                             | false, false => d
+                                             end |> cekValue_of_integer |> Some
+   | _                                    => None
+   end.
+
+Definition modInteger (Vs : list cekValue) : option cekValue :=
+   match Vs with
+   | [VCon (Integer a); VCon (Integer 0)] => None
+   | [VCon (Integer a); VCon (Integer b)] => let m := Z.abs (Z.modulo a b) in
+                                             match a >=? 0, b >=? 0 with
+                                             | true , true  => m
+                                             | false, true  => m
+                                             | true , false => m
+                                             | false, false => -m
+                                             end |> cekValue_of_integer |> Some
+   | _                                    => None
+   end.
+
+Definition quotientInteger (Vs : list cekValue) : option cekValue :=
+   match Vs with
+   | [VCon (Integer a); VCon (Integer 0)] => None
+   | [VCon (Integer a); VCon (Integer b)] => let q := Z.abs (Z.quot a b) in
+                                             match a >=? 0, b >=? 0 with
+                                             | true , true  => q
+                                             | false, true  => -q
+                                             | true , false => q
+                                             | false, false => q
+                                             end |> cekValue_of_integer |> Some
+   | _                                    => None
+   end.
+
+Definition remainderInteger (Vs : list cekValue) : option cekValue :=
+   match Vs with
+   | [VCon (Integer a); VCon (Integer 0)] => None
+   | [VCon (Integer a); VCon (Integer b)] => let r := Z.abs (Z.rem a b) in
+                                             match a >=? 0, b >=? 0 with
+                                             | true , true  => r
+                                             | false, true  => -r
+                                             | true , false => r
+                                             | false, false => -r
+                                             end |> cekValue_of_integer |> Some
+   | _                                    => None
+   end.
+
+Definition equalsInteger (Vs : list cekValue) : option cekValue :=
+  match Vs with
+   | [VCon (Integer x); VCon (Integer y)] => Some (cekValue_of_boolean (x =? y))
    | _                                    => None
    end.
 
 Definition lessThanInteger (Vs : list cekValue) : option cekValue :=
   match Vs with
-   | [VCon (Integer x); VCon (Integer y)] => Some (VCon (Bool (x <=? y)))
+   | [VCon (Integer x); VCon (Integer y)] => Some (cekValue_of_boolean (x <? y))
    | _                                    => None
+   end.
+
+Definition lessThanEqualsInteger (Vs : list cekValue) : option cekValue :=
+  match Vs with
+   | [VCon (Integer x); VCon (Integer y)] => Some (cekValue_of_boolean (x <=? y))
+   | _                                    => None
+   end.
+
+Local Definition exp_mod (a : Z) (e m : positive) : Z := a ^ (Zpos e) mod (Zpos m).
+
+Local Definition exp_mod_inverse (a : Z) (e m' : positive) : option Z :=
+  let m := Zpos m' in
+  match Z.gcd a m with
+  | 1 => Some ((a ^ (Zpos e)) ^ (m - 2) mod m)
+  | _ => None
+  end.
+
+Definition expModInteger (Vs : list cekValue) : option cekValue :=
+  match Vs with
+   | [VCon (Integer a); VCon (Integer  Z0     ); VCon (Integer (Zpos m))] => 1             |> cekValue_of_integer |> Some
+   | [VCon (Integer a); VCon (Integer (Zpos e)); VCon (Integer (Zpos m))] => exp_mod a e m |> cekValue_of_integer |> Some
+   | [VCon (Integer a); VCon (Integer (Zneg e)); VCon (Integer (Zpos m))] => option_map (cekValue_of_integer) (exp_mod_inverse a e m)
+   | _                                                                    => None
    end.
