theories/PlutusV3/BuiltinFunctions/List.v
@@ -1,0 +1,41 @@
+From Coq Require Import Lists.List.
+                 Import ListNotations.
+
+From CoqUplc Require Import Prelude.FunctionalNotations.
+
+From CoqUplc Require Import PlutusV3.CekValue.
+From CoqUplc Require Import PlutusV3.Uplc.
+
+Local Open Scope functional_scope.
+
+Definition chooseList (Vs : list cekValue) : option cekValue :=
+   match Vs with
+   | [VCon (ConstList []); nil_case; _        ] => Some nil_case
+   | [VCon (ConstList _ ); _       ; cons_case] => Some cons_case
+   | _                                          => None
+   end.
+
+Definition mkCons (Vs : list cekValue) : option cekValue :=
+   match Vs with
+   | [VCon x; VCon (ConstList xs)] => x :: xs |> cekValue_of_list |> Some
+   | _                             => None
+   end.
+
+Definition headList (Vs : list cekValue) : option cekValue :=
+   match Vs with
+   | [VCon (ConstList (x :: _))] => x |> VCon |> Some
+   | _                           => None
+   end.
+
+Definition tailList (Vs : list cekValue) : option cekValue :=
+   match Vs with
+   | [VCon (ConstList (_ :: xs))] => xs |> cekValue_of_list |> Some
+   | _                            => None
+   end.
+
+Definition nullList (Vs : list cekValue) : option cekValue :=
+   match Vs with
+   | [VCon (ConstList [])] => true  |> cekValue_of_boolean |> Some
+   | [VCon (ConstList _ )] => false |> cekValue_of_boolean |> Some
+   | _                     => None
+   end.
