theories/PlutusV3/BuiltinFunctions/Misc.v
@@ -1,0 +1,22 @@
+From Coq Require Import Lists.List.
+                 Import ListNotations.
+
+From CoqUplc Require Import Prelude.List.
+From CoqUplc Require Import Prelude.Monad.
+                     Import MonadNotations.
+
+From CoqUplc Require Import PlutusV3.CekValue.
+From CoqUplc Require Import PlutusV3.Uplc.
+From CoqUplc Require Import Unicode.String.
+
+Definition chooseUnit (Vs : list cekValue) : option cekValue :=
+   match Vs with
+   | [VCon Unit; val] => Some val
+   | _                => None
+   end.
+
+Definition trace (Vs : list cekValue) : writer (list unicodestring) (option cekValue) :=
+  match Vs with
+  | [VCon (ConstString x); val] => (tell [x] ;; mreturn (Some val))%monad
+  | _                           => mreturn None
+  end.
