theories/PlutusV3/BuiltinFunctions/Pair.v
@@ -1,0 +1,17 @@
+From Coq Require Import Lists.List.
+                 Import ListNotations.
+
+From CoqUplc Require Import PlutusV3.CekValue.
+From CoqUplc Require Import PlutusV3.Uplc.
+
+Definition fstPair (Vs : list cekValue) : option cekValue :=
+   match Vs with
+   | [VCon (Pair x _)] => Some (VCon x)
+   | _                 => None
+   end.
+
+Definition sndPair (Vs : list cekValue) : option cekValue :=
+   match Vs with
+   | [VCon (Pair _ y)] => Some (VCon y)
+   | _                 => None
+   end.
