theories/PlutusV3/BuiltinFunctions/String.v
@@ -1,0 +1,36 @@
+From Coq Require Import Lists.List.
+                 Import ListNotations.
+
+From CoqUplc Require Import Prelude.FunctionalNotations.
+
+From CoqUplc Require Import PlutusV3.CekValue.
+From CoqUplc Require Import PlutusV3.Uplc.
+From CoqUplc Require Import Unicode.String.
+From CoqUplc Require Import Unicode.Utf8Encoding.
+
+Local Open Scope string_scope.
+Local Open Scope functional_scope.
+
+Definition appendString (Vs : list cekValue) : option cekValue :=
+   match Vs with
+   | [VCon (ConstString x); VCon (ConstString y)] => append x y |> cekValue_of_string |> Some
+   | _                                            => None
+   end.
+
+Definition equalsString (Vs : list cekValue) : option cekValue :=
+   match Vs with
+   | [VCon (ConstString x); VCon (ConstString y)] => eqb x y |> cekValue_of_boolean |> Some
+   | _                                            => None
+   end.
+
+Definition encodeUtf8 (Vs : list cekValue) : option cekValue :=
+   match Vs with
+   | [VCon (ConstString x)] => option_map cekValue_of_byteString (encode_utf8 x)
+   | _                      => None
+   end.
+
+Definition decodeUtf8 (Vs : list cekValue) : option cekValue :=
+   match Vs with
+   | [VCon (ByteString x)] => option_map cekValue_of_string (decode_utf8 x)
+   | _                     => None
+   end.
