theories/PlutusV3/CekValue.v
@@ -1,15 +1,30 @@
 From Coq Require Import Strings.String.
+From Coq Require Import ZArith.
+
+From CoqUplc Require Import Prelude.FunctionalNotations.
 
 From CoqUplc Require Import PlutusV3.Builtins.
 From CoqUplc Require Import PlutusV3.Uplc.
+From CoqUplc Require Import Unicode.String.
 
 Inductive cekValue : Set :=
   | VCon     : const                                              -> cekValue
   | VDelay   :           term -> environment                      -> cekValue
   | VLam     : string -> term -> environment                      -> cekValue
-  | VConstr  : nat        -> list cekValue                        -> cekValue
+  | VConstr  : N          -> list cekValue                        -> cekValue
   | VBuiltin : builtinFun -> list cekValue -> expectedBuiltinArgs -> cekValue
 
 with environment : Set :=
   | NonEmptyEnvironment : environment -> string -> cekValue -> environment
   | EmptyEnvironment    :                                      environment.
+
+Local Open Scope functional_scope.
+
+Definition cekValue_of_integer    (x : Z)             : cekValue := Integer     x |> VCon.
+Definition cekValue_of_byteString (x : string)        : cekValue := ByteString  x |> VCon.
+Definition cekValue_of_string     (x : unicodestring) : cekValue := ConstString x |> VCon.
+Definition cekValue_of_unit                           : cekValue :=          Unit |> VCon.
+Definition cekValue_of_boolean    (x : bool)          : cekValue := Bool        x |> VCon.
+Definition cekValue_of_list       (x : list const)    : cekValue := ConstList   x |> VCon.
+Definition cekValue_of_pair       (x y : const)       : cekValue := Pair      x y |> VCon.
+Definition cekValue_of_data       (x : data)          : cekValue := Data        x |> VCon.
