theories/Prelude/Bytes.v
@@ -1,0 +1,301 @@
+From Coq Require Import FunInd.
+From Coq Require Import funind.Recdef.
+From Coq Require Import Lists.List.
+                 Import ListNotations.
+From Coq Require Import Strings.Ascii.
+From Coq Require Import Strings.String.
+From Coq Require Import NArith.
+From Coq Require Import ZArith.
+
+From CoqUplc Require Import Prelude.FunctionalNotations.
+From CoqUplc Require Import Prelude.Option.
+
+Local Open Scope functional_scope.
+Local Open Scope positive_scope.
+
+Local Fixpoint bit_list_of_pos_le (p : positive) {struct p} : list bool :=
+  match p with
+  | p ~ 1 => true  :: bit_list_of_pos_le p
+  | p ~ 0 => false :: bit_list_of_pos_le p
+  | xH    => [true]
+  end.
+
+Local Example bit_list_of_pos_le_ex1 : bit_list_of_pos_le 15 = [ true; true;  true; true]. Proof eq_refl.
+Local Example bit_list_of_pos_le_ex2 : bit_list_of_pos_le 10 = [false; true; false; true]. Proof eq_refl.
+
+
+Local Definition bytestring_of_pos_le (p : positive) : string :=
+  let bit_list_le := bit_list_of_pos_le p in
+  (fix loop (l : list bool) {struct l} : string :=
+    match l with
+    | b0 :: b1 :: b2 :: b3 :: b4 :: b5 :: b6 :: b7 :: t => String (Ascii b0 b1    b2    b3    b4    b5    b6    b7   ) (loop t)
+    | b0 :: b1 :: b2 :: b3 :: b4 :: b5 :: b6 :: nil     => String (Ascii b0 b1    b2    b3    b4    b5    b6    false) EmptyString
+    | b0 :: b1 :: b2 :: b3 :: b4 :: b5 :: nil           => String (Ascii b0 b1    b2    b3    b4    b5    false false) EmptyString
+    | b0 :: b1 :: b2 :: b3 :: b4 :: nil                 => String (Ascii b0 b1    b2    b3    b4    false false false) EmptyString
+    | b0 :: b1 :: b2 :: b3 :: nil                       => String (Ascii b0 b1    b2    b3    false false false false) EmptyString
+    | b0 :: b1 :: b2 :: nil                             => String (Ascii b0 b1    b2    false false false false false) EmptyString
+    | b0 :: b1 :: nil                                   => String (Ascii b0 b1    false false false false false false) EmptyString
+    | b0 :: nil                                         => String (Ascii b0 false false false false false false false) EmptyString
+    | nil                                               => EmptyString
+    end) bit_list_le.
+
+Local Example bytestring_of_pos_le_ex1 : bytestring_of_pos_le   15 = string_of_list_ascii ["015"%char].             Proof eq_refl.
+Local Example bytestring_of_pos_le_ex2 : bytestring_of_pos_le 1234 = string_of_list_ascii ["210"%char; "004"%char]. Proof eq_refl.
+
+
+Definition bytestring_of_N_le (n : N) : string :=
+  match n with
+  | N0     => ""%string
+  | Npos p => bytestring_of_pos_le p
+  end.
+
+Definition bytestring_of_N_be (n : N) : string := n |> bytestring_of_N_le |> list_ascii_of_string |> @rev ascii |> string_of_list_ascii.
+
+
+Local Open Scope Z_scope.
+Local Open Scope bool_scope.
+
+Local Fixpoint replicate (a : ascii) (n : nat) : string :=
+  match n with
+  | O   => EmptyString
+  | S p => String a (replicate a p)
+  end.
+
+Local Definition pad_string_left (s : string) (w : nat) : string :=
+  concat "" [replicate "000"%char (w - length s); s].
+
+Local Definition pad_string_right (s : string) (w : nat) : string :=
+  concat "" [s; replicate "000"%char (w - length s)].
+
+Local Example pad_string_left_ex  : pad_string_left  "12"%string 4 = string_of_list_ascii ["000"%char; "000"%char; "1"%char; "2"%char]. Proof eq_refl.
+Local Example pad_string_rigth_ex : pad_string_right "12"%string 4 = string_of_list_ascii ["1"%char; "2"%char; "000"%char; "000"%char]. Proof eq_refl.
+
+Definition integer_to_bytestring (e : bool) (w n : Z) : option string :=
+  let w_in_range := (0 <=? w) && (w <=? 8192       ) in
+  let n_in_range := (0 <=? n) && (n <?  Z.pow 256 w) in
+  match w_in_range && n_in_range, e with
+  | true , true  => (* big-endian *)
+      let bs := n |> Z.to_N |> bytestring_of_N_be in
+      if w =? 0 then Some bs
+                else Some (pad_string_left bs (w |> Z.to_nat))
+  | true , false => (* little-endian *)
+      let bs := n |> Z.to_N |> bytestring_of_N_le in
+      if w =? 0 then Some bs
+                else Some (pad_string_right bs (w |> Z.to_nat))
+  | false, _     => None
+  end.
+
+
+Fixpoint bytestring_to_integer_le (s : string) {struct s} : N :=
+  match s with
+  | EmptyString => 0
+  | String a t  => (N_of_ascii a) + 256 * (bytestring_to_integer_le t)
+  end.
+
+Local Example bytestring_to_integer_le_ex1 : bytestring_to_integer_le "cafe"%string = 1701208419%N. Proof eq_refl.
+
+Fixpoint bytestring_to_integer_be (s : string) (acc : N) {struct s} : N :=
+  match s with
+  | EmptyString => acc
+  | String a t  => bytestring_to_integer_be t ((N_of_ascii a) + acc * 256)
+  end.
+
+Local Example bytestring_to_integer_be_ex1 : bytestring_to_integer_be "efac"%string 0 = 1701208419%N. Proof eq_refl.
+
+Definition bytestring_to_integer (e : bool) (s : string) : N :=
+  match e with
+  | true  => bytestring_to_integer_be s 0
+  | false => bytestring_to_integer_le s
+  end.
+
+
+Local Close Scope Z_scope.
+Local Close Scope positive_scope.
+
+Definition truncate_to (s : string) (k : nat)             : string := substring 0 k s.
+Definition extend_to   (s : string) (k : nat) (a : ascii) : string := append s (replicate a (k - length s)).
+
+Local Definition and_ascii (a b : ascii) : ascii :=
+  let (a0, a1, a2, a3, a4, a5, a6, a7) := a in
+  let (b0, b1, b2, b3, b4, b5, b6, b7) := b in
+  Ascii (andb a0 b0) (andb a1 b1) (andb a2 b2) (andb a3 b3) (andb a4 b4) (andb a5 b5) (andb a6 b6) (andb a7 b7).
+
+Local Definition or_ascii (a b : ascii) : ascii :=
+  let (a0, a1, a2, a3, a4, a5, a6, a7) := a in
+  let (b0, b1, b2, b3, b4, b5, b6, b7) := b in
+  Ascii (orb a0 b0) (orb a1 b1) (orb a2 b2) (orb a3 b3) (orb a4 b4) (orb a5 b5) (orb a6 b6) (orb a7 b7).
+
+Local Definition xor_ascii (a b : ascii) : ascii :=
+  let (a0, a1, a2, a3, a4, a5, a6, a7) := a in
+  let (b0, b1, b2, b3, b4, b5, b6, b7) := b in
+  Ascii (xorb a0 b0) (xorb a1 b1) (xorb a2 b2) (xorb a3 b3) (xorb a4 b4) (xorb a5 b5) (xorb a6 b6) (xorb a7 b7).
+
+Local Fixpoint string_map2 (f : ascii -> ascii -> ascii) (s1 s2 : string) {struct s1} : string :=
+  match s1, s2 with
+  | EmptyString  , _             => EmptyString
+  | _            , EmptyString   => EmptyString
+  | String a1 s1', String a2 s2' => String (f a1 a2) (string_map2 f s1' s2')
+  end.
+
+Local Definition loop_over_strings (f : ascii -> ascii -> ascii) (e : bool) (a : ascii) (s1 s2 : string) : string :=
+  match e with
+  | false => let l := Nat.min (length s1) (length s2) in string_map2 f (truncate_to s1 l) (truncate_to s2 l)
+  | true  => let l := Nat.max (length s1) (length s2) in string_map2 f (extend_to s1 l a) (extend_to s2 l a)
+  end.
+
+Definition and_bytestring (e : bool) (s1 s2 : string) : string := loop_over_strings and_ascii e "255"%char s1 s2.
+Definition  or_bytestring (e : bool) (s1 s2 : string) : string := loop_over_strings or_ascii  e "000"%char s1 s2.
+Definition xor_bytestring (e : bool) (s1 s2 : string) : string := loop_over_strings xor_ascii e "000"%char s1 s2.
+
+
+Local Fixpoint bytestring_to_bits (s : string) {struct s} : list bool :=
+  match s with
+  | String (Ascii b0 b1 b2 b3 b4 b5 b6 b7) t => b7 :: b6 :: b5 :: b4 :: b3 :: b2 :: b1 :: b0 :: bytestring_to_bits t
+  | EmptyString                              => []
+  end.
+
+Local Example bytestring_to_bits_ex1 : bytestring_to_bits " "%string = [false; false; true; false; false; false; false; false]. Proof eq_refl.
+
+Local Fixpoint bytestring_of_bits (l : list bool) : string :=
+  match l with
+  | b0 :: b1 :: b2 :: b3 :: b4 :: b5 :: b6 :: b7 :: t => String (Ascii b7    b6    b5    b4    b3    b2    b1    b0   ) (bytestring_of_bits t)
+  | b0 :: b1 :: b2 :: b3 :: b4 :: b5 :: b6 :: nil     => String (Ascii b6    b5    b4    b3    b2    b1    b0    false) EmptyString
+  | b0 :: b1 :: b2 :: b3 :: b4 :: b5 :: nil           => String (Ascii b5    b4    b3    b2    b1    b0    false false) EmptyString
+  | b0 :: b1 :: b2 :: b3 :: b4 :: nil                 => String (Ascii b4    b3    b2    b1    b0    false false false) EmptyString
+  | b0 :: b1 :: b2 :: b3 :: nil                       => String (Ascii b3    b2    b1    b0    false false false false) EmptyString
+  | b0 :: b1 :: b2 :: nil                             => String (Ascii b2    b1    b0    false false false false false) EmptyString
+  | b0 :: b1 :: nil                                   => String (Ascii b1    b0    false false false false false false) EmptyString
+  | b0 :: nil                                         => String (Ascii b0    false false false false false false false) EmptyString
+  | nil                                               => EmptyString
+  end.
+
+Local Example bytestring_of_bits_ex1 : bytestring_of_bits [true; false; false; false; false; false] = " "%string. Proof eq_refl.
+
+Local Theorem bytestring_bits_bytestring : forall s, (s |> bytestring_to_bits |> bytestring_of_bits) = s.
+Proof.
+  induction s as [|a t IHs].
+  - reflexivity.
+  - destruct a as [b0 b1 b2 b3 b4 b5 b6 b7] eqn: Ea; simpl; repeat rewrite <- Ea; now rewrite IHs.
+Qed.
+
+
+Definition shift_bits_left (s : string) (k : nat) : string :=
+  let b  := bytestring_to_bits s            in
+  let b' := skipn k (b ++ (repeat false k)) in
+  bytestring_of_bits b'.
+
+(* "ca" = x63 x61 = 0110 0011  0110 0001 *)
+(*        xC6 xC2 = 1100 0110  1100 0010 *)
+Local Example shift_bits_left_ex1 : shift_bits_left "ca"%string  1 = string_of_list_ascii ["198"%char; "194"%char]. Proof eq_refl.
+Local Example shift_bits_left_ex2 : shift_bits_left "ca"%string  8 = string_of_list_ascii [  "a"%char; "000"%char]. Proof eq_refl.
+Local Example shift_bits_left_ex3 : shift_bits_left "ca"%string 16 = string_of_list_ascii ["000"%char; "000"%char]. Proof eq_refl.
+Local Example shift_bits_left_ex4 : shift_bits_left   ""%string 24 = ""%string. Proof eq_refl.
+
+Definition shift_bits_right (s : string) (k : nat) : string :=
+  let b  := bytestring_to_bits s                           in
+  let b' := firstn (List.length b) ((repeat false k) ++ b) in
+  bytestring_of_bits b'.
+
+(* "ca" = x63 x61 = 0110 0011  0110 0001 *)
+(*        x31 xB0 = 0011 0001  1011 0000 *)
+Local Example shift_bits_right_ex1 : shift_bits_right "ca"%string  1 = string_of_list_ascii ["049"%char; "176"%char]. Proof eq_refl.
+Local Example shift_bits_right_ex2 : shift_bits_right "ca"%string  8 = string_of_list_ascii ["000"%char;   "c"%char]. Proof eq_refl.
+Local Example shift_bits_right_ex3 : shift_bits_right "ca"%string 16 = string_of_list_ascii ["000"%char; "000"%char]. Proof eq_refl.
+Local Example shift_bits_right_ex4 : shift_bits_right   ""%string  2 = ""%string. Proof eq_refl.
+
+Definition rotate_bits_left (s : string) (k : nat) : string :=
+  let b  := bytestring_to_bits s          in
+  let k' := Nat.modulo k (List.length b)  in
+  let b' := skipn k' (b ++ (firstn k' b)) in
+  bytestring_of_bits b'.
+
+(* "ca" = x63 x61 = 0110 0011  0110 0001 *)
+(*        xC6 xC2 = 1100 0110  1100 0010 *)
+Local Example rotate_bits_left_ex1 : rotate_bits_left "ca"%string  1 = string_of_list_ascii ["198"%char; "194"%char]. Proof eq_refl.
+Local Example rotate_bits_left_ex2 : rotate_bits_left "ca"%string  8 = "ac"%string. Proof eq_refl.
+Local Example rotate_bits_left_ex3 : rotate_bits_left "ca"%string 16 = "ca"%string. Proof eq_refl.
+Local Example rotate_bits_left_ex4 : rotate_bits_left "ca"%string 24 = "ac"%string. Proof eq_refl.
+Local Example rotate_bits_left_ex5 : rotate_bits_left   ""%string 32 =  ""%string. Proof eq_refl.
+
+Definition rotate_bits_right (s : string) (k : nat) : string :=
+  let b  := bytestring_to_bits s                      in
+  let k' := Nat.modulo k (List.length b)              in
+  let n  := List.length b - k'                        in
+  let b' := firstn (List.length b) ((skipn n b) ++ b) in
+  bytestring_of_bits b'.
+
+(* "ca" = x63 x61 = 0110 0011  0110 0001 *)
+(*        xB1 xB0 = 1011 0001  1011 0000 *)
+Local Example rotate_bits_right_ex1 : rotate_bits_right "ca"%string  1 = string_of_list_ascii ["177"%char; "176"%char]. Proof eq_refl.
+Local Example rotate_bits_right_ex2 : rotate_bits_right "ca"%string  8 = "ac"%string. Proof eq_refl.
+Local Example rotate_bits_right_ex3 : rotate_bits_right "ca"%string 16 = "ca"%string. Proof eq_refl.
+Local Example rotate_bits_right_ex4 : rotate_bits_right "ca"%string 24 = "ac"%string. Proof eq_refl.
+Local Example rotate_bits_right_ex5 : rotate_bits_right   ""%string  7 =   ""%string. Proof eq_refl.
+
+Definition count_set_bits (s : string) : nat := count_occ Bool.bool_dec (bytestring_to_bits s) true.
+
+Local Fixpoint find_index {A : Type} (f : A -> bool) (l : list A) : option nat :=
+  match l with
+  | h :: t => if f h then Some 0 else option_map (Nat.add 1) (find_index f t)
+  | []     => None
+  end.
+
+Definition first_set_bit (s : string) : Z :=
+  match find_index id (s |> bytestring_to_bits |> @rev bool) with
+  | Some x => x |> Z.of_nat
+  | None   => -1
+  end.
+
+Local Example first_set_bit_ex1 : first_set_bit " "%string = 5%Z. Proof eq_refl.
+
+Definition read_bit (s : string) (n : nat) : option bool :=
+  let b := (s |> bytestring_to_bits |> @rev bool) in
+  nth_error b n.
+
+Local Example read_bit_ex1 : read_bit " "%string 5 = Some true. Proof eq_refl.
+
+
+Local Fixpoint update_bit (b : list bool) (n : nat) (u : bool) {struct b} : option (list bool) :=
+  match b, n with
+  | h :: t, 0   => Some (u :: t)
+  | h :: t, S p => option_map (cons h) (update_bit t p u)
+  | []    , _   => None
+  end.
+
+Local Example update_bit_ex1 : update_bit [true; true; true; true] 2 false = Some [true; true; false; true]. Proof eq_refl.
+
+Local Theorem update_bits_spec1 : forall b n u, n < List.length b -> update_bit b n u = Some (firstn n b ++ [u] ++ skipn (n + 1) b).
+Proof.
+  induction b as [|h t IHb].
+  - simpl; intros n u Hn; contradict Hn; unfold lt; apply Nat.nle_succ_0. 
+  - induction n as [|p IHp]; try reflexivity; simpl; intros u HSp; rewrite IHb.
+    + reflexivity.
+    + now apply PeanoNat.lt_S_n.
+Qed.
+
+Local Theorem update_bits_spec2 : forall b n u, List.length b <= n -> update_bit b n u = None.
+Proof.
+  induction b as [|h t IHb]; try reflexivity; induction n as [|p IHp]; simpl; intros u Hl.
+  - contradict Hl; apply Nat.nle_succ_0. 
+  - rewrite IHb; [reflexivity | now apply le_S_n].
+Qed.
+
+Fixpoint update_bits (j : list Z) (u : bool) (b : list bool) {struct j} : option (list bool) :=
+  match j with
+  | Zpos p :: t => option_flatmap (update_bits t u) (update_bit b (Pos.to_nat p) u)
+  | Z0     :: t => option_flatmap (update_bits t u) (update_bit b 0              u)
+  | Zneg _ :: _ => None
+  | []          => Some b
+  end.
+
+Definition write_bits (s : string) (u : bool) (j : list Z) : option string :=
+  let r := update_bits j u (s |> bytestring_to_bits |> @rev bool) in
+  option_map (@rev bool >> bytestring_of_bits) r.
+
+
+Local Open Scope Z_scope.
+
+Definition replicate_bytes (l b : Z) : option string :=
+       if (l <? 0) || (8192 <? l) then None
+  else if (b <? 0) || ( 255 <? b) then None
+  else replicate (b |> Z.to_N |> ascii_of_N) (l |> Z.to_nat) |> Some.
