theories/Prelude/List.v
@@ -1,0 +1,11 @@
+From Coq Require Import Lists.List.
+
+From CoqUplc Require Import Prelude.Monad.
+
+Instance semigroup_list {A : Type} : Semigroup (list A) := {
+  sconcat := fun a b => app a b
+}.
+
+Instance monoid_list {A : Type} : Monoid (list A) _ := {
+  mempty := nil
+}.
