theories/Prelude/Monad.v
@@ -1,0 +1,33 @@
+
+Class Semigroup (A : Type) := {
+  sconcat : A -> A -> A
+}.
+
+Class Monoid (A : Type) `(S : Semigroup A) := {
+  mempty : A
+}.
+
+Class Monad (M : Type -> Type) := {
+  mbind   : forall {A B : Type}, M A -> (A -> M B) -> M B
+; mreturn : forall {A   : Type}, A -> M A
+}.
+
+Module MonadNotations.
+  Declare Scope monad_scope.
+  Delimit Scope monad_scope with monad.
+
+  Notation "x <- m1 ;; m2" := (mbind m1 (fun x => m2)) (at level  75, right associativity, m1 at next level) : monad_scope.
+  Notation      "m1 ;; m2" := (mbind m1 (fun _ => m2)) (at level 100, right associativity)                   : monad_scope.
+End MonadNotations.
+
+Inductive writer (W A : Type) := Writer (a : A) (w : W).
+
+Instance monad_writer {W : Type} `{Monoid W} : Monad (writer W) := {
+  mbind   := fun {A} {B} ma f => let (a, w0) := ma  in
+                                 let (b, w1) := f a in
+                                 Writer W B b (sconcat w0 w1)
+; mreturn := fun {A} a => Writer W A a mempty
+}.
+
+Definition tell {W : Type} (w : W) : writer W unit :=
+  Writer W unit tt w.
