theories/Prelude/Show.v
@@ -11,27 +11,26 @@ Class Show (A : Type) := {
   show : A -> string
 }.
 
-#[export]
 Instance show_uint : Show uint := {
   show := NilZero.string_of_uint
 }.
 
-#[export]
 Instance show_int : Show int := {
   show := NilZero.string_of_int
 }.
 
-#[export]
 Instance show_nat : Show nat := {
   show n := show (to_uint n)
 }.
 
-#[export]
 Instance show_Z : Show Z := {
   show z := show (Z.to_int z)
 }.
 
-#[export]
+Instance show_N : Show N := {
+  show n := show (N.to_int n)
+}.
+
 Instance show_bool : Show bool := {
   show b := if b then "true" else "false"
 }.
@@ -39,7 +38,6 @@ Instance show_bool : Show bool := {
 Definition showList {A : Type} (f : A -> string) (xs : list A) : string :=
   "[" ++ (concat "; " (map f xs)) ++ "]".
 
-#[export]
 Instance show_list {A : Type} `{Show A} : Show (list A) := {
   show := showList show
 }.
@@ -47,7 +45,6 @@ Instance show_list {A : Type} `{Show A} : Show (list A) := {
 Definition showPair {A B : Type} (fa : A -> string) (fb : B -> string) (p : A * B) : string :=
   let (a, b) := p in "(" ++ fa a ++ ", " ++ fb b ++ ")".
 
-#[export]
 Instance show_pair {A B : Type} `{Show A} `{Show B} : Show (A * B) := {
   show := showPair show show
 }.
