theories/Unicode/String.v
@@ -1,0 +1,33 @@
+From Coq Require Import NArith.
+From Coq Require Import Lists.List.
+                 Import ListNotations.
+
+From CoqUplc Require Import Prelude.Monad.
+
+Inductive unicodestring : Set := Unicode (chars : list N).
+
+Definition append (a b : unicodestring) : unicodestring :=
+  let (a') := a in
+  let (b') := b in
+  Unicode (app a' b').
+
+Fixpoint eqb_list (a b : list N) {struct a} : bool :=
+  match a, b with
+  | [], []             => true
+  | [], _              => false
+  | _ , []             => false
+  | ha :: ta, hb :: tb => andb (N.eqb ha hb) (eqb_list ta tb)
+  end.
+
+Definition eqb (a b : unicodestring) : bool :=
+  let (a') := a in
+  let (b') := b in
+  eqb_list a' b'.
+
+Instance semigroup_unicodestring : Semigroup unicodestring := {
+  sconcat := fun a b => append a b
+}.
+
+Instance monoid_unicodestring : Monoid unicodestring _ := {
+  mempty := Unicode []
+}.
