theories/Unicode/StringShow.v
@@ -1,0 +1,26 @@
+From Coq Require Import Init.Byte.
+From Coq Require Import Strings.String.
+
+From CoqUplc Require Import Prelude.Show.
+From CoqUplc Require Import Unicode.String.
+From CoqUplc Require Import Unicode.Utf8Encoding.
+
+Instance show_unicodestring : Show unicodestring := {
+  show u :=
+    match encode_utf8 u with
+    | Some s => "Unicode """ ++ s ++ """"
+    | None   => "Unicode: message utf8 encoding error"
+    end
+}.
+
+Definition parse_unicodestring (x : list byte) : option unicodestring :=
+  decode_utf8 (string_of_list_byte x).
+
+Definition print_unicodestring (x : unicodestring) : option (list byte) :=
+  option_map (list_byte_of_string) (encode_utf8 x).
+
+Declare Scope unicode_scope.
+Delimit Scope unicode_scope with unicode.
+
+String Notation unicodestring parse_unicodestring print_unicodestring : unicode_scope.
+
