theories/Unicode/Utf8Encoding.v
@@ -1,0 +1,151 @@
+From Coq Require Import Lists.List.
+                 Import ListNotations.
+From Coq Require Import NArith.
+From Coq Require Import Strings.Ascii.
+From Coq Require Import Strings.String.
+
+From CoqUplc Require Import Prelude.FunctionalNotations.
+From CoqUplc Require Import Prelude.Option.
+
+From CoqUplc Require Import Unicode.String.
+
+Local Open Scope N_scope.
+Local Open Scope functional_scope.
+
+Definition get_bits_4 (n : N) :=
+  [N.testbit n 3; N.testbit n 2; N.testbit n 1; N.testbit n 0].
+
+Local Notation "x !! y" := (nth y x false) (at level 99).
+Local Notation "x +: y" := (String x y)    (at level 99, right associativity).
+
+Local Definition create_byte (b : list bool) : ascii :=
+  (Ascii (b !! 7) (b !! 6) (b !! 5) (b !! 4) (b !! 3) (b !! 2) (b !! 1) (b !! 0))%nat.
+
+Local Example create_byte_ex1 : create_byte [false; true; true; false; false; false; false; true] = "a"%char. Proof eq_refl.
+
+
+Local Definition encode_char_1 (n : N) : string :=
+  String (ascii_of_N (N.modulo n 0x0080)) EmptyString.
+
+Local Example encode_char_1_ex1 : encode_char_1  86 = "V"%string. Proof eq_refl.
+Local Example encode_char_1_ex2 : encode_char_1 342 = "V"%string. Proof eq_refl.
+
+
+Local Definition encode_char_2 (n : N) : string :=
+  let x     := N.modulo (N.div n 0x100) 0x10 in
+  let y     := N.modulo (N.div n  0x10) 0x10 in
+  let z     := N.modulo n               0x10 in
+  let xxxx  := get_bits_4 x                  in
+  let yyyy  := get_bits_4 y                  in
+  let zzzz  := get_bits_4 z                  in
+  let byte1 := create_byte [true;  true;     false; xxxx !! 1;  xxxx !! 2; xxxx !! 3; yyyy !! 0; yyyy !! 1] in
+  let byte2 := create_byte [true; false; yyyy !! 2; yyyy !! 3;  zzzz !! 0; zzzz !! 1; zzzz !! 2; zzzz !! 3] in
+  byte1 +: byte2 +: "".
+
+Local Example encode_char_2_ex1 : encode_char_2 961 = "ρ"%string. Proof eq_refl.
+
+
+Local Definition encode_char_3 (n : N) : string :=
+  let w     := N.modulo (N.div n 0x1000) 0x10 in
+  let x     := N.modulo (N.div n  0x100) 0x10 in
+  let y     := N.modulo (N.div n   0x10) 0x10 in
+  let z     := N.modulo n                0x10 in
+  let wwww  := get_bits_4 w                   in
+  let xxxx  := get_bits_4 x                   in
+  let yyyy  := get_bits_4 y                   in
+  let zzzz  := get_bits_4 z                   in
+  let byte1 := create_byte [true;  true;     true; false;       wwww !! 0; wwww !! 1; wwww !! 2; wwww !! 3] in
+  let byte2 := create_byte [true; false; xxxx !! 0; xxxx !! 1;  xxxx !! 2; xxxx !! 3; yyyy !! 0; yyyy !! 1] in
+  let byte3 := create_byte [true; false; yyyy !! 2; yyyy !! 3;  zzzz !! 0; zzzz !! 1; zzzz !! 2; zzzz !! 3] in
+  byte1 +: byte2 +: byte3 +: "".
+
+Local Example encode_char_3_ex1 : encode_char_3 0x13EB = "Ꮻ"%string. Proof eq_refl.
+
+
+Local Definition encode_char_4 (n : N) : string :=
+  let u     := N.modulo (N.div n 0x100000) 0x10 in
+  let v     := N.modulo (N.div n  0x10000) 0x10 in
+  let w     := N.modulo (N.div n   0x1000) 0x10 in
+  let x     := N.modulo (N.div n    0x100) 0x10 in
+  let y     := N.modulo (N.div n     0x10) 0x10 in
+  let z     := N.modulo n                  0x10 in
+  let uuuu  := get_bits_4 u                     in
+  let vvvv  := get_bits_4 v                     in
+  let wwww  := get_bits_4 w                     in
+  let xxxx  := get_bits_4 x                     in
+  let yyyy  := get_bits_4 y                     in
+  let zzzz  := get_bits_4 z                     in
+  let byte1 := create_byte [true;  true;     true;  true;           false; uuuu !! 3; vvvv !! 0; vvvv !! 1] in
+  let byte2 := create_byte [true; false; vvvv !! 2; vvvv !! 3;  wwww !! 0; wwww !! 1; wwww !! 2; wwww !! 3] in
+  let byte3 := create_byte [true; false; xxxx !! 0; xxxx !! 1;  xxxx !! 2; xxxx !! 3; yyyy !! 0; yyyy !! 1] in
+  let byte4 := create_byte [true; false; yyyy !! 2; yyyy !! 3;  zzzz !! 0; zzzz !! 1; zzzz !! 2; zzzz !! 3] in
+  byte1 +: byte2 +: byte3 +: byte4 +: "".
+
+Local Example encode_char_4_ex1 : encode_char_4 0x1D11E = "𝄞"%string. Proof eq_refl.
+
+
+Local Definition encode_char (n : N) : option string :=
+       if n <?   0x007F then Some (encode_char_1 n)
+  else if n <?   0x07FF then Some (encode_char_2 n)
+  else if n <?   0xFFFF then Some (encode_char_3 n)
+  else if n <? 0x10FFFF then Some (encode_char_4 n)
+  else None.
+
+Local Example encode_char_ex1 : encode_char 0x10C8D = Some ("𐲍"%string). Proof eq_refl.
+
+
+Definition encode_utf8 (u : unicodestring) : option string :=
+  let (charcodes) := u                     in
+  let append'     := Strings.String.append in
+  fold_left (fun a b => option_map2 append' a (encode_char b)) charcodes (Some EmptyString).
+
+Local Example encode_utf8_ex1 : encode_utf8 (Unicode [])                        = Some (      ""%string). Proof eq_refl.
+Local Example encode_utf8_ex2 : encode_utf8 (Unicode [52; 50])                  = Some (    "42"%string). Proof eq_refl.
+Local Example encode_utf8_ex3 : encode_utf8 (Unicode [961; 32; 0x25B7; 32; 77]) = Some ("ρ ▷ M"%string). Proof eq_refl.
+
+
+Local Definition decode_char_1 := N_of_ascii.
+
+Local Definition decode_char_2 (a b : ascii) : N :=
+  let (y1, y0, x2, x1, x0, _ , _, _) := a in
+  let (z3, z2, z1, z0, y3, y2, _, _) := b in
+  N_of_digits [z3; z2; z1; z0; y3; y2; y1; y0; x2; x1; x0].
+
+Local Example decode_char_2_ex1 : decode_char_2 (ascii_of_N 207) (ascii_of_N 129) = 961. Proof eq_refl.
+
+
+Local Definition decode_char_3 (a b c : ascii) : N :=
+  let (w3, w2, w1, w0, _ , _ , _, _) := a in
+  let (y1, y0, x3, x2, x1, x0, _, _) := b in
+  let (z3, z2, z1, z0, y3, y2, _, _) := c in
+  N_of_digits [z3; z2; z1; z0; y3; y2; y1; y0; x3; x2; x1; x0; w3; w2; w1; w0].
+
+Local Example decode_char_3_ex1 : decode_char_3 (ascii_of_N 225) (ascii_of_N 143) (ascii_of_N 171) = 0x13EB. Proof eq_refl.
+
+
+Local Definition decode_char_4 (a b c d : ascii) : N :=
+  let (v1, v0, u0, _ , _ , _ , _, _) := a in
+  let (w3, w2, w1, w0, v3, v2, _, _) := b in
+  let (y1, y0, x3, x2, x1, x0, _, _) := c in
+  let (z3, z2, z1, z0, y3, y2, _, _) := d in
+  N_of_digits [z3; z2; z1; z0; y3; y2; y1; y0; x3; x2; x1; x0; w3; w2; w1; w0; v3; v2; v1; v0; u0].
+
+Local Example decode_char_4_ex1 : decode_char_4 (ascii_of_N 240) (ascii_of_N 157) (ascii_of_N 132) (ascii_of_N 158) = 0x1D11E. Proof eq_refl.
+
+
+Local Fixpoint decode_chars (a : string) (acc : list N) (n : nat) {struct n} : option (list N) :=
+  let drop n := substring n (length a) a in
+  match n, a with
+  | S p, String (Ascii _ _ _ _     _     _     _    false) _ => option_flatmap  (decode_char_1 >>    (fun r => decode_chars (drop 1%nat) (r :: acc) p)) (get 0 a)
+  | S p, String (Ascii _ _ _ _     _     false true true ) _ => option_flatmap2 (decode_char_2 >>>   (fun r => decode_chars (drop 2%nat) (r :: acc) p)) (get 0 a) (get 1 a)
+  | S p, String (Ascii _ _ _ _     false true  true true ) _ => option_flatmap3 (decode_char_3 >>>>  (fun r => decode_chars (drop 3%nat) (r :: acc) p)) (get 0 a) (get 1 a) (get 2 a)
+  | S p, String (Ascii _ _ _ false true  true  true true ) _ => option_flatmap4 (decode_char_4 >>>>> (fun r => decode_chars (drop 4%nat) (r :: acc) p)) (get 0 a) (get 1 a) (get 2 a) (get 3 a)
+  | _,   EmptyString                                         => Some (rev acc)
+  | _,   _                                                   => None
+  end.
+
+
+Definition decode_utf8 (s : string) : option unicodestring :=
+  option_map (fun u => Unicode u) (decode_chars s [] (length s)).
+
+Local Example decode_utf8_ex1 : decode_utf8 "𐲍"%string = Some (Unicode [0x10C8D]). Proof eq_refl.
